add refframe and prove trace for add

theories/example.v
@@ -1,5 +1,5 @@
 Require Import isla.base.
-Require Import isla.isla_lang.
+Require Import isla.opsem.
 
 (* trace of add x1, x2, x3:
   (read-reg |R2| nil v3359)
@@ -15,14 +15,38 @@ Require Import isla.isla_lang.
 *)
 Definition add_x1_x2_x3 : trc :=
   [
+  Smt (DeclareConst 3359 (Ty_BitVec 64)) Mk_annot;
+  Smt (DeclareConst 3361 (Ty_BitVec 64)) Mk_annot;
   ReadReg "R2" [] (Val_Symbolic 3359) Mk_annot;
-  Smt (DefineConst 3425 (Var 3359 Mk_annot)) Mk_annot;
+  Smt (DefineConst 3425 (Val (Val_Symbolic 3359) Mk_annot)) Mk_annot;
   ReadReg "R3" [] (Val_Symbolic 3361) Mk_annot;
-  Smt (DefineConst 3426 (Var 3361 Mk_annot)) Mk_annot;
-  Smt (DefineConst 3431 (Unop (ZeroExtend 64) (Var 3425 Mk_annot) Mk_annot)) Mk_annot;
-  Smt (DefineConst 3432 (Unop (ZeroExtend 64) (Var 3426 Mk_annot) Mk_annot)) Mk_annot;
-  Smt (DefineConst 3433 (Manyop (Bvmanyarith Bvadd) [Var 3431 Mk_annot; Var 3432 Mk_annot] Mk_annot)) Mk_annot;
-  Smt (DefineConst 3437 (Unop (Extract 63 0) (Var 3433 Mk_annot) Mk_annot)) Mk_annot;
-  Smt (DefineConst 3452 (Var 3467 Mk_annot)) Mk_annot;
-  WriteReg "R1" [] (Val_Symbolic 3453) Mk_annot
+  Smt (DefineConst 3426 (Val (Val_Symbolic 3361) Mk_annot)) Mk_annot;
+  Smt (DefineConst 3431 (Unop (ZeroExtend 64) (Val (Val_Symbolic 3425) Mk_annot) Mk_annot)) Mk_annot;
+  Smt (DefineConst 3432 (Unop (ZeroExtend 64) (Val (Val_Symbolic 3426) Mk_annot) Mk_annot)) Mk_annot;
+  Smt (DefineConst 3433 (Manyop (Bvmanyarith Bvadd) [Val (Val_Symbolic 3431) Mk_annot; Val (Val_Symbolic 3432) Mk_annot] Mk_annot)) Mk_annot;
+  Smt (DefineConst 3437 (Unop (Extract 63 0) (Val (Val_Symbolic 3433) Mk_annot) Mk_annot)) Mk_annot;
+  Smt (DefineConst 3452 (Val (Val_Symbolic 3437) Mk_annot)) Mk_annot;
+  WriteReg "R1" [] (Val_Symbolic 3452) Mk_annot
 ].
+
+Lemma add_x1_x2_x3_trace bv2 bv3 :
+  add_x1_x2_x3 ~{ trace_module, [
+                    Vis (LReadReg "R2" [] (Val_Bits bv2));
+                    Vis (LReadReg "R3" [] (Val_Bits bv3));
+                    Vis (LWriteReg "R1" [] (Val_Bits (Z_extract 63 0 (bv2 + bv3))))
+                ] }~> [].
+Proof.
+  apply: TraceStepNone. { apply: (DeclareConstS (Val_Bits _)). shelve. } simpl.
+  apply: TraceStepNone. { apply: (DeclareConstS (Val_Bits _)). shelve. } simpl.
+  apply: TraceStepSome. { econstructor. } simpl.
+  apply: TraceStepNone. { by econstructor. } simpl.
+  apply: TraceStepSome. { econstructor. } simpl.
+  apply: TraceStepNone. { by econstructor. } simpl.
+  apply: TraceStepNone. { by econstructor. } simpl.
+  apply: TraceStepNone. { by econstructor. } simpl.
+  apply: TraceStepNone. { by econstructor. } simpl.
+  apply: TraceStepNone. { by econstructor. } simpl.
+  apply: TraceStepNone. { by econstructor. } simpl.
+  apply: TraceStepSome. { econstructor. } simpl.
+  by apply: TraceEnd.
+Qed.
